src/Lean/Meta/Tactic/Grind/Arith/Cutsat/Util.lean
@@ -60,7 +60,7 @@ def getVar (x : Var) : GoalM Expr :=
   return (← get').vars[x]!
 
 /-- Returns `true` if `e` is already associated with a cutsat variable. -/
-def isVar (e : Expr) : GoalM Bool :=
+def hasVar (e : Expr) : GoalM Bool :=
   return (← get').varMap.contains { expr := e }
 
 /-- Returns `true` if `x` has been eliminated using an equality constraint. -/
